src/MicroSail/Context.v
@@ -1,0 +1,123 @@
+(******************************************************************************)
+(* Copyright (c) 2019 Steven Keuchel                                          *)
+(* All rights reserved.                                                       *)
+(*                                                                            *)
+(* Redistribution and use in source and binary forms, with or without         *)
+(* modification, are permitted provided that the following conditions are     *)
+(* met:                                                                       *)
+(*                                                                            *)
+(* 1. Redistributions of source code must retain the above copyright notice,  *)
+(*    this list of conditions and the following disclaimer.                   *)
+(*                                                                            *)
+(* 2. Redistributions in binary form must reproduce the above copyright       *)
+(*    notice, this list of conditions and the following disclaimer in the     *)
+(*    documentation and/or other materials provided with the distribution.    *)
+(*                                                                            *)
+(* THIS SOFTWARE IS PROVIDED BY THE COPYRIGHT HOLDERS AND CONTRIBUTORS        *)
+(* "AS IS" AND ANY EXPRESS OR IMPLIED WARRANTIES, INCLUDING, BUT NOT LIMITED  *)
+(* TO, THE IMPLIED WARRANTIES OF MERCHANTABILITY AND FITNESS FOR A PARTICULAR *)
+(* PURPOSE ARE DISCLAIMED. IN NO EVENT SHALL THE COPYRIGHT HOLDER OR          *)
+(* CONTRIBUTORS BE LIABLE FOR ANY DIRECT, INDIRECT, INCIDENTAL, SPECIAL,      *)
+(* EXEMPLARY, OR CONSEQUENTIAL DAMAGES (INCLUDING, BUT NOT LIMITED TO,        *)
+(* PROCUREMENT OF SUBSTITUTE GOODS OR SERVICES; LOSS OF USE, DATA, OR         *)
+(* PROFITS; OR BUSINESS INTERRUPTION) HOWEVER CAUSED AND ON ANY THEORY OF     *)
+(* LIABILITY, WHETHER IN CONTRACT, STRICT LIABILITY, OR TORT (INCLUDING       *)
+(* NEGLIGENCE OR OTHERWISE) ARISING IN ANY WAY OUT OF THE USE OF THIS         *)
+(* SOFTWARE, EVEN IF ADVISED OF THE POSSIBILITY OF SUCH DAMAGE.               *)
+(******************************************************************************)
+
+Require Import Coq.Logic.EqdepFacts.
+
+Set Implicit Arguments.
+
+(* Type of contexts. This is a list of bindings of type B. This type and
+   subsequent types use the common notation of snoc lists. *)
+Inductive Ctx (B : Set) : Set :=
+| ctx_nil
+| ctx_snoc (Γ : Ctx B) (b : B).
+
+Arguments ctx_nil {_}.
+Arguments ctx_snoc {_} _ _.
+
+Section WithBinding.
+  Context {B : Set}.
+
+  (* Concatenation of two contexts. *)
+  Fixpoint ctx_cat (Γ1 Γ2 : Ctx B) {struct Γ2} : Ctx B :=
+    match Γ2 with
+    | ctx_nil       => Γ1
+    | ctx_snoc Γ2 τ => ctx_snoc (ctx_cat Γ1 Γ2) τ
+    end.
+
+  (* This is a predicate that that encodes that the de Bruijn index n points
+     to the binding b in Γ. *)
+  Fixpoint ctx_nth_is (Γ : Ctx B) (n : nat) (b : B) {struct Γ} : Prop :=
+    match Γ , n with
+    | ctx_snoc _ x , O   => x = b
+    | ctx_snoc Γ _ , S n => ctx_nth_is Γ n b
+    | _            , _   => False
+    end.
+
+  Section InCtx.
+    (* Set locally only for the definition of InCtx. *)
+    Local Set Primitive Projections.
+
+     (* InCtx represents context containment proofs. This is essentially a
+        well-typed de Bruijn index, i.e. a de Bruijn index with a proof that it
+        resolves to the binding b. This record type is defined using primitive
+        projections to get eta-conversion definitionally. *)
+    Class InCtx (b : B) (Γ : Ctx B) : Set :=
+      { inctx_at: nat;
+        inctx_valid: ctx_nth_is Γ inctx_at b
+      }.
+  End InCtx.
+
+  (* These are *constructors* for InCtx. *)
+  Definition inctx_zero {b : B} {Γ : Ctx B} : InCtx b (ctx_snoc Γ b) :=
+    Build_InCtx b (ctx_snoc Γ b) 0 eq_refl.
+  Definition inctx_succ {b : B} {Γ : Ctx B} {b' : B} (bIn : InCtx b Γ) :
+    InCtx b (ctx_snoc Γ b') :=
+    Build_InCtx b (ctx_snoc Γ b') (S inctx_at) inctx_valid.
+
+  (* Custom pattern matching in cases where the context was already refined
+     by a different match, i.e. on environments. *)
+  Definition inctx_case_nil {b : B} {A : Set} (bIn : InCtx b ctx_nil) : A :=
+    let (n, e) := bIn in match e with end.
+  Definition inctx_case_snoc (D : B -> Set) (Γ : Ctx B) (b0 : B) (db0 : D b0)
+    (dΓ: forall b, InCtx b Γ -> D b) (b : B) (bIn: InCtx b (ctx_snoc Γ b0)) : D b :=
+    let (n, e) := bIn in
+    match n return ctx_nth_is (ctx_snoc Γ b0) n b -> D b with
+    | 0 =>   eq_rec b0 D db0 b
+    | S n => fun e => dΓ b (Build_InCtx _ _ n e)
+    end e.
+
+  Definition inctx_case_snoc_dep (Γ : Ctx B) (b0 : B)
+    (D : forall b, InCtx b (ctx_snoc Γ b0) -> Prop)
+    (db0 : D b0 inctx_zero)
+    (dΓ: forall b (bIn: InCtx b Γ), D b (inctx_succ bIn)) :
+    forall (y: B) (yIn: InCtx y (ctx_snoc Γ b0)), D y yIn :=
+    fun b bIn =>
+      match bIn with
+        Build_InCtx _ _ n e =>
+        match n return forall e, D b (Build_InCtx _ _ n e) with
+        | 0 => eq_indd B b0 (fun z e => D z (Build_InCtx _ (ctx_snoc _ _) 0 e)) db0 b
+        | S n => fun e => dΓ b (Build_InCtx _ _ n e)
+        end e
+      end.
+
+  Lemma InCtx_ind (b : B)
+    (P : forall (Γ : Ctx B), InCtx b Γ -> Prop)
+    (fzero : forall (Γ : Ctx B), P (ctx_snoc Γ b) inctx_zero)
+    (fsucc : forall (Γ : Ctx B) (b0 : B) (bIn : InCtx b Γ),
+        P Γ bIn -> P (ctx_snoc Γ b0) (inctx_succ bIn)) :
+    forall (Γ : Ctx B) (bIn : InCtx b Γ), P Γ bIn.
+  Proof.
+    induction Γ; cbn.
+    - intro bIn; exact (inctx_case_nil bIn).
+    - intros [[|n] e]; cbn in *.
+      + subst; apply fzero.
+      + pose (Build_InCtx _ _ n e) as bIn.
+        exact (fsucc Γ _ bIn (IHΓ bIn)).
+  Qed.
+
+End WithBinding.
